make a defaults file to simplify examples in Bedrock/Tests

src/Bedrock/Tests/X25519_64.v
@@ -7,6 +7,7 @@ Require Import Coq.Lists.List.
 Require Import Crypto.BoundsPipeline.
 Require Import Crypto.Arithmetic.Core.
 Require Import Crypto.Arithmetic.ModOps.
+Require Import Crypto.Bedrock.Defaults.
 Require Import Crypto.Bedrock.Types.
 Require Import Crypto.Bedrock.Translation.Func.
 Require Import Crypto.Language.API.
@@ -19,10 +20,13 @@ Require bedrock2.NotationsCustomEntry.
 
 Import Language.Compilers.
 Import Associational Positional.
-Import Types.Notations.
+Import Types.Notations Defaults.Notations.
 
 Require Import Crypto.Util.Notations.
 Import ListNotations. Local Open Scope Z_scope.
+Local Open Scope string_scope.
+Local Open Scope expr_scope.
+Local Open Scope core_scope.
 
 Local Coercion Z.of_nat : nat >-> Z.
 Local Coercion QArith_base.inject_Z : Z >-> Q.
@@ -33,34 +37,10 @@ Module X25519_64.
   Section __.
     Context (n : nat := 5%nat)
             (s : Z := 2^255)
-            (c : list (Z * Z) := [(1,19)])
-            (machine_wordsize : Z := 64).
-
-    Local Existing Instance default_low_level_rewriter_method.
-    (* Split multiplications into two outputs, not just one huge word *)
-    Local Instance should_split_mul : should_split_mul_opt := true.
-    (* For functions that return multiple values, split into two LetIns (this is
-       because bedrock2 does not support multiple-sets, so they would have to be
-       split anyway) *)
-    Local Instance should_split_multiret : should_split_multiret_opt := true.
-    (* Make all words 64-bit, even if they could be smaller *)
-    Local Instance widen_carry : widen_carry_opt := true.
-    Local Instance widen_bytes : widen_bytes_opt := true.
-    (* Unsigned integers *)
-    Local Instance only_signed : only_signed_opt := false.
+            (c : list (Z * Z) := [(1,19)]%list).
 
     Let limbwidth := (Z.log2_up (s - Associational.eval c) / Z.of_nat n)%Q.
     Let idxs := (List.seq 0 n ++ [0; 1])%list%nat.
-
-    Definition possible_values_of_machine_wordsize
-      := prefix_with_carry [machine_wordsize; 2 * machine_wordsize]%Z.
-
-    Let possible_values := possible_values_of_machine_wordsize.
-
-    Local Instance split_mul_to : split_mul_to_opt :=
-      split_mul_to_of_should_split_mul machine_wordsize possible_values.
-    Local Instance split_multiret_to : split_multiret_to_opt :=
-      split_multiret_to_of_should_split_multiret machine_wordsize possible_values.
 
     Let prime_upperbound_list : list Z
       := encode_no_reduce (weight (Qnum limbwidth) (Qden limbwidth)) n (s-1).
@@ -76,16 +56,6 @@ Module X25519_64.
     Definition limbwidth_num := Eval vm_compute in Qnum limbwidth.
     Definition limbwidth_den := Eval vm_compute in QDen limbwidth.
 
-    Set Printing Depth 100000.
-    Local Open Scope string_scope.
-    Local Notation "'uint64,uint64'" := (ident.Literal
-                                           (r[0 ~> 18446744073709551615]%zrange,
-                                            r[0 ~> 18446744073709551615]%zrange)%core) : expr_scope.
-    Local Notation "'uint64'" :=
-      (ident.Literal (t:=Compilers.zrange) r[0 ~> 18446744073709551615]%zrange) : expr_scope.
-    Local Open Scope expr_scope.
-    Local Open Scope core_scope.
-
     Definition mulmod_ : Pipeline.ErrorT (Expr _) :=
       Pipeline.BoundsPipeline
         false (* subst01 *)
@@ -100,20 +70,6 @@ Module X25519_64.
            As mulmod_eq.
     Proof. vm_compute; reflexivity. Qed.
 
-    Local Existing Instances Types.rep.Z Types.rep.listZ_mem.
-    Let wordsize_bytes := Eval vm_compute in (machine_wordsize / 8)%Z.
-
-    Local Definition ERROR := "ERROR".
-    Instance p : Types.parameters :=
-      {| semantics := BasicC64Semantics.parameters;
-         varname_gen := fun i => String.append "x" (Decimal.decimal_string_of_Z (Z.of_nat i));
-         error := expr.var ERROR;
-         word_size_in_bytes := wordsize_bytes;
-      |}.
-
-    Definition bedrock_func : Type :=
-      string * (list string * list string * cmd.cmd).
-
     Definition mulmod_bedrock : bedrock_func :=
       ("mulmod_bedrock",
        translate_func mulmod
@@ -121,28 +77,6 @@ Module X25519_64.
                       (n, (n, tt)) (* lengths for list arguments *)
                       "out0" (* return value name *)).
 
-    (* quick check to make sure the expression produced no errors *)
-    Fixpoint error_free_expr (x : Syntax.expr) : bool :=
-      match x with
-      | expr.literal _ => true
-      | expr.var x => negb (String.eqb x ERROR)
-      | expr.load _ a => error_free_expr a
-      | expr.op _ x y => (error_free_expr x && error_free_expr y)%bool
-      end.
-    Fixpoint error_free_cmd (x : cmd.cmd) : bool :=
-      match x with
-      | cmd.skip => true
-      | cmd.unset _ => true 
-      | cmd.set _ v => error_free_expr v
-      | cmd.store _ a v =>
-        (error_free_expr a && error_free_expr v)%bool
-      | cmd.cond c t f =>
-        (error_free_expr c && error_free_cmd t && error_free_cmd f)%bool
-      | cmd.seq x y => (error_free_cmd x && error_free_cmd y)%bool
-      | cmd.while c b => (error_free_expr c && error_free_cmd b)
-      | cmd.call _ _ args => forallb error_free_expr args
-      | cmd.interact _ _ args => forallb error_free_expr args
-      end.
     Goal (error_free_cmd (snd (snd mulmod_bedrock)) = true).
     Proof. vm_compute. reflexivity. Qed.
 
