src/Bedrock/Defaults.v
@@ -1,0 +1,92 @@
+Require Import Coq.ZArith.ZArith.
+Require Import Coq.Strings.String.
+Require Import Coq.Lists.List.
+Require Import bedrock2.Syntax.
+Require Import bedrock2.Semantics.
+Require Import bedrock2.BasicC64Semantics.
+Require Import Crypto.Bedrock.Types.
+Require Import Crypto.BoundsPipeline.
+Require Import Crypto.Language.API.
+Require Import Crypto.Util.ZRange.
+Import API.Compilers.
+
+Require Import Crypto.Util.Notations.
+Import Types.Notations ListNotations.
+Local Open Scope Z_scope.
+Local Open Scope string_scope.
+
+(* Declares default parameters for the bedrock2 backend and includes useful
+   definitions/proofs that apply specifically to the defaults. Do NOT import
+   this file unless you're prepared to have a bunch of global typeclass
+   instances and notations declared for you. *)
+
+Section Defaults.
+  Definition machine_wordsize := 64.
+
+  (* Reification/bounds pipeline options *)
+  Global Existing Instance default_low_level_rewriter_method.
+  (* Split multiplications into two outputs, not just one huge word *)
+  Global Instance should_split_mul : should_split_mul_opt := true.
+  (* For functions that return multiple values, split into two LetIns (this is
+     because bedrock2 does not support multiple-sets, so they would have to be
+     split anyway) *)
+  Global Instance should_split_multiret : should_split_multiret_opt := true.
+  (* Make all words 64-bit, even if they could be smaller *)
+  Global Instance widen_carry : widen_carry_opt := true.
+  Global Instance widen_bytes : widen_bytes_opt := true.
+  (* Unsigned integers *)
+  Global Instance only_signed : only_signed_opt := false.
+
+  (* Define how to split mul/multi-return functions *)
+  Definition possible_values
+    := prefix_with_carry [machine_wordsize; 2 * machine_wordsize]%Z.
+  Global Instance split_mul_to : split_mul_to_opt :=
+    split_mul_to_of_should_split_mul machine_wordsize possible_values.
+  Global Instance split_multiret_to : split_multiret_to_opt :=
+    split_multiret_to_of_should_split_multiret machine_wordsize possible_values.
+
+  (* bedrock2 backend parameters *)
+  Global Existing Instances Types.rep.Z Types.rep.listZ_mem.
+  Let wordsize_bytes := Eval vm_compute in (machine_wordsize / 8)%Z.
+  Local Definition ERROR := "ERROR".
+  Global Instance default_parameters : Types.parameters :=
+    {| semantics := BasicC64Semantics.parameters;
+       varname_gen := fun i => String.append "x" (Decimal.decimal_string_of_Z (Z.of_nat i));
+       error := expr.var ERROR;
+       word_size_in_bytes := wordsize_bytes;
+    |}.
+
+  Definition bedrock_func : Type :=
+    string * (list string * list string * cmd.cmd).
+
+  (* quick check to make sure the expression produced no errors *)
+  Fixpoint error_free_expr (x : Syntax.expr) : bool :=
+    match x with
+    | expr.literal _ => true
+    | expr.var x => negb (String.eqb x ERROR)
+    | expr.load _ a => error_free_expr a
+    | expr.op _ x y => (error_free_expr x && error_free_expr y)%bool
+    end.
+  Fixpoint error_free_cmd (x : cmd.cmd) : bool :=
+    match x with
+    | cmd.skip => true
+    | cmd.unset _ => true 
+    | cmd.set _ v => error_free_expr v
+    | cmd.store _ a v =>
+      (error_free_expr a && error_free_expr v)%bool
+    | cmd.cond c t f =>
+      (error_free_expr c && error_free_cmd t && error_free_cmd f)%bool
+    | cmd.seq x y => (error_free_cmd x && error_free_cmd y)%bool
+    | cmd.while c b => (error_free_expr c && error_free_cmd b)
+    | cmd.call _ _ args => forallb error_free_expr args
+    | cmd.interact _ _ args => forallb error_free_expr args
+    end.
+End Defaults.
+
+Module Notations.
+  Notation "'uint64,uint64'" := (ident.Literal
+                                   (r[0 ~> 18446744073709551615]%zrange,
+                                    r[0 ~> 18446744073709551615]%zrange)%core) : expr_scope.
+  Notation "'uint64'" :=
+    (ident.Literal (t:=Compilers.zrange) r[0 ~> 18446744073709551615]%zrange) : expr_scope.
+End Notations.
